syntax/SLoopStride.v
@@ -8,6 +8,15 @@ Definition stride_loop :
     SPolIRs.Loop.stmt :=
   CoreStride.stride_loop.
 
+Definition down_stride_loop :
+    nat -> SPolIRs.Loop.expr -> SPolIRs.Loop.expr -> SPolIRs.Loop.stmt ->
+    SPolIRs.Loop.stmt :=
+  CoreStride.down_stride_loop.
+
 Definition stride_count_expr :
     nat -> SPolIRs.Loop.expr -> SPolIRs.Loop.expr -> SPolIRs.Loop.expr :=
   CoreStride.stride_count_expr.
+
+Definition down_stride_count_expr :
+    nat -> SPolIRs.Loop.expr -> SPolIRs.Loop.expr -> SPolIRs.Loop.expr :=
+  CoreStride.down_stride_count_expr.
